coq_translation/axiomatized/examples/std_library_types/result.v
@@ -10,23 +10,6 @@ Module checked.
   End MathError.
   Definition MathError := MathError.t.
   
-  Module Impl_core_fmt_Debug_for_result_checked_MathError.
-    Definition Self := result.checked.MathError.
-    
-    Parameter fmt : forall `{H : State.Trait},
-        ref Self ->
-        mut_ref core.fmt.Formatter ->
-        M (H := H) core.fmt.Result.
-    
-    Global Instance Method_fmt `{H : State.Trait} : Notation.Dot "fmt" := {
-      Notation.dot := fmt;
-    }.
-    
-    Global Instance I : core.fmt.Debug.Trait Self := {
-      core.fmt.Debug.fmt `{H : State.Trait} := fmt;
-    }.
-  End Impl_core_fmt_Debug_for_result_checked_MathError.
-  
   Definition MathResult : Set :=
     core.result.Result f64 result.checked.MathError.
   
