CoqOfRust/ink/ink_env.v
@@ -949,7 +949,7 @@ Module api.
       `{ink_env.types.Environment.Trait E}
       `{ink_env.call.create_builder.FromAccountId.Trait E ContractRef}
       `{parity_scale_codec.codec.Encode.Trait Args}
-      `{core.convert.AsRef.Trait (Slice u8) Salt}
+      `{core.convert.AsRef.Trait Slice Salt}
       `{ink_env.call.create_builder.ConstructorReturnType.Trait ContractRef R}
       ref
         (ink_env.call.create_builder.CreateParams E ContractRef Args Salt R) ->
@@ -995,7 +995,7 @@ Module api.
       forall
       {H : Set},
       `{ink_env.hash.CryptoHash.Trait H}
-      ref (Slice u8) ->
+      ref Slice ->
       mut_ref ink_env.hash.HashOutput.Type ->
       M (H := H) unit.
   
@@ -1202,7 +1202,7 @@ Parameter instantiate_contract : forall `{H : State.Trait},
     `{ink_env.types.Environment.Trait E}
     `{ink_env.call.create_builder.FromAccountId.Trait E ContractRef}
     `{parity_scale_codec.codec.Encode.Trait Args}
-    `{core.convert.AsRef.Trait (Slice u8) Salt}
+    `{core.convert.AsRef.Trait Slice Salt}
     `{ink_env.call.create_builder.ConstructorReturnType.Trait ContractRef R}
     ref (ink_env.call.create_builder.CreateParams E ContractRef Args Salt R) ->
     M (H := H)
@@ -1245,7 +1245,7 @@ Parameter hash_bytes : forall `{H : State.Trait},
     forall
     {H : Set},
     `{ink_env.hash.CryptoHash.Trait H}
-    ref (Slice u8) ->
+    ref Slice ->
     mut_ref ink_env.hash.HashOutput.Type ->
     M (H := H) unit.
 
@@ -1890,7 +1890,7 @@ Module backend.
         `{H : State.Trait}
         :
         (mut_ref Self) ->
-        (ref (Slice u8)) ->
+        (ref Slice) ->
         (mut_ref ink_env.hash.HashOutput.Type) ->
         (M (H := H) unit);
       hash_encoded
@@ -1928,7 +1928,7 @@ Module backend.
         `{H : State.Trait}
         :
         (mut_ref Self) ->
-        (ref (Slice u8)) ->
+        (ref Slice) ->
         (M (H := H) (ink_env.error.Result unit));
     }.
     
@@ -2457,7 +2457,7 @@ Module EnvBackend.
       `{H : State.Trait}
       :
       (mut_ref Self) ->
-      (ref (Slice u8)) ->
+      (ref Slice) ->
       (mut_ref ink_env.hash.HashOutput.Type) ->
       (M (H := H) unit);
     hash_encoded
@@ -2494,9 +2494,7 @@ Module EnvBackend.
     set_code_hash
       `{H : State.Trait}
       :
-      (mut_ref Self) ->
-      (ref (Slice u8)) ->
-      (M (H := H) (ink_env.error.Result unit));
+      (mut_ref Self) -> (ref Slice) -> (M (H := H) (ink_env.error.Result unit));
   }.
   
   Global Instance Method_set_contract_storage `{H : State.Trait} `(Trait)
@@ -11338,7 +11336,7 @@ Module engine.
         
         Parameter params : forall `{H : State.Trait},
             ref Self ->
-            M (H := H) (ref (Slice u8)).
+            M (H := H) (ref Slice).
         
         Global Instance Method_params `{H : State.Trait} :
           Notation.Dot "params" := {
@@ -11347,7 +11345,7 @@ Module engine.
         
         Parameter to_bytes : forall `{H : State.Trait},
             ref Self ->
-            M (H := H) (ref (Slice u8)).
+            M (H := H) (ref Slice).
         
         Global Instance Method_to_bytes `{H : State.Trait} :
           Notation.Dot "to_bytes" := {
@@ -11410,7 +11408,7 @@ Module engine.
         Definition Self := ink_env.hash.Blake2x128.
         
         Parameter hash : forall `{H : State.Trait},
-            ref (Slice u8) ->
+            ref Slice ->
             mut_ref ink_env.hash.HashOutput.Type ->
             M (H := H) unit.
         
@@ -11428,7 +11426,7 @@ Module engine.
         Definition Self := ink_env.hash.Blake2x256.
         
         Parameter hash : forall `{H : State.Trait},
-            ref (Slice u8) ->
+            ref Slice ->
             mut_ref ink_env.hash.HashOutput.Type ->
             M (H := H) unit.
         
@@ -11446,7 +11444,7 @@ Module engine.
         Definition Self := ink_env.hash.Sha2x256.
         
         Parameter hash : forall `{H : State.Trait},
-            ref (Slice u8) ->
+            ref Slice ->
             mut_ref ink_env.hash.HashOutput.Type ->
             M (H := H) unit.
         
@@ -11464,7 +11462,7 @@ Module engine.
         Definition Self := ink_env.hash.Keccak256.
         
         Parameter hash : forall `{H : State.Trait},
-            ref (Slice u8) ->
+            ref Slice ->
             mut_ref ink_env.hash.HashOutput.Type ->
             M (H := H) unit.
         
@@ -11591,9 +11589,7 @@ Module engine.
         
         Parameter get_property : forall `{H : State.Trait},
             mut_ref Self ->
-            (ref ink_engine.ext.Engine) ->
-            (mut_ref (mut_ref (Slice u8))) ->
-            unit ->
+            (ref ink_engine.ext.Engine) -> (mut_ref (mut_ref Slice)) -> unit ->
             M (H := H) (ink_env.error.Result T).
         
         Global Instance Method_get_property `{H : State.Trait} :
@@ -11689,7 +11685,7 @@ Module engine.
         
         Parameter hash_bytes : forall `{H : State.Trait},
             mut_ref Self ->
-            ref (Slice u8) ->
+            ref Slice ->
             mut_ref ink_env.hash.HashOutput.Type ->
             M (H := H) unit.
         
@@ -11747,7 +11743,7 @@ Module engine.
         
         Parameter set_code_hash : forall `{H : State.Trait},
             mut_ref Self ->
-            ref (Slice u8) ->
+            ref Slice ->
             M (H := H) (ink_env.error.Result unit).
         
         Global Instance Method_set_code_hash `{H : State.Trait} :
@@ -12819,7 +12815,7 @@ Module off_chain.
       
       Parameter params : forall `{H : State.Trait},
           ref Self ->
-          M (H := H) (ref (Slice u8)).
+          M (H := H) (ref Slice).
       
       Global Instance Method_params `{H : State.Trait} :
         Notation.Dot "params" := {
@@ -12828,7 +12824,7 @@ Module off_chain.
       
       Parameter to_bytes : forall `{H : State.Trait},
           ref Self ->
-          M (H := H) (ref (Slice u8)).
+          M (H := H) (ref Slice).
       
       Global Instance Method_to_bytes `{H : State.Trait} :
         Notation.Dot "to_bytes" := {
@@ -12891,7 +12887,7 @@ Module off_chain.
       Definition Self := ink_env.hash.Blake2x128.
       
       Parameter hash : forall `{H : State.Trait},
-          ref (Slice u8) ->
+          ref Slice ->
           mut_ref ink_env.hash.HashOutput.Type ->
           M (H := H) unit.
       
@@ -12909,7 +12905,7 @@ Module off_chain.
       Definition Self := ink_env.hash.Blake2x256.
       
       Parameter hash : forall `{H : State.Trait},
-          ref (Slice u8) ->
+          ref Slice ->
           mut_ref ink_env.hash.HashOutput.Type ->
           M (H := H) unit.
       
@@ -12927,7 +12923,7 @@ Module off_chain.
       Definition Self := ink_env.hash.Sha2x256.
       
       Parameter hash : forall `{H : State.Trait},
-          ref (Slice u8) ->
+          ref Slice ->
           mut_ref ink_env.hash.HashOutput.Type ->
           M (H := H) unit.
       
@@ -12945,7 +12941,7 @@ Module off_chain.
       Definition Self := ink_env.hash.Keccak256.
       
       Parameter hash : forall `{H : State.Trait},
-          ref (Slice u8) ->
+          ref Slice ->
           mut_ref ink_env.hash.HashOutput.Type ->
           M (H := H) unit.
       
@@ -13066,9 +13062,7 @@ Module off_chain.
       
       Parameter get_property : forall `{H : State.Trait},
           mut_ref Self ->
-          (ref ink_engine.ext.Engine) ->
-          (mut_ref (mut_ref (Slice u8))) ->
-          unit ->
+          (ref ink_engine.ext.Engine) -> (mut_ref (mut_ref Slice)) -> unit ->
           M (H := H) (ink_env.error.Result T).
       
       Global Instance Method_get_property `{H : State.Trait} :
@@ -13164,7 +13158,7 @@ Module off_chain.
       
       Parameter hash_bytes : forall `{H : State.Trait},
           mut_ref Self ->
-          ref (Slice u8) ->
+          ref Slice ->
           mut_ref ink_env.hash.HashOutput.Type ->
           M (H := H) unit.
       
@@ -13222,7 +13216,7 @@ Module off_chain.
       
       Parameter set_code_hash : forall `{H : State.Trait},
           mut_ref Self ->
-          ref (Slice u8) ->
+          ref Slice ->
           M (H := H) (ink_env.error.Result unit).
       
       Global Instance Method_set_code_hash `{H : State.Trait} :
@@ -14232,7 +14226,7 @@ Module call_data.
     
     Parameter params : forall `{H : State.Trait},
         ref Self ->
-        M (H := H) (ref (Slice u8)).
+        M (H := H) (ref Slice).
     
     Global Instance Method_params `{H : State.Trait} :
       Notation.Dot "params" := {
@@ -14241,7 +14235,7 @@ Module call_data.
     
     Parameter to_bytes : forall `{H : State.Trait},
         ref Self ->
-        M (H := H) (ref (Slice u8)).
+        M (H := H) (ref Slice).
     
     Global Instance Method_to_bytes `{H : State.Trait} :
       Notation.Dot "to_bytes" := {
@@ -14435,7 +14429,7 @@ Module Impl_ink_env_engine_off_chain_call_data_CallData_4.
   
   Parameter params : forall `{H : State.Trait},
       ref Self ->
-      M (H := H) (ref (Slice u8)).
+      M (H := H) (ref Slice).
   
   Global Instance Method_params `{H : State.Trait} : Notation.Dot "params" := {
     Notation.dot := params;
@@ -14443,7 +14437,7 @@ Module Impl_ink_env_engine_off_chain_call_data_CallData_4.
   
   Parameter to_bytes : forall `{H : State.Trait},
       ref Self ->
-      M (H := H) (ref (Slice u8)).
+      M (H := H) (ref Slice).
   
   Global Instance Method_to_bytes `{H : State.Trait} :
     Notation.Dot "to_bytes" := {
@@ -14503,7 +14497,7 @@ Module impls.
     Definition Self := ink_env.hash.Blake2x128.
     
     Parameter hash : forall `{H : State.Trait},
-        ref (Slice u8) ->
+        ref Slice ->
         mut_ref ink_env.hash.HashOutput.Type ->
         M (H := H) unit.
     
@@ -14521,7 +14515,7 @@ Module impls.
     Definition Self := ink_env.hash.Blake2x256.
     
     Parameter hash : forall `{H : State.Trait},
-        ref (Slice u8) ->
+        ref Slice ->
         mut_ref ink_env.hash.HashOutput.Type ->
         M (H := H) unit.
     
@@ -14539,7 +14533,7 @@ Module impls.
     Definition Self := ink_env.hash.Sha2x256.
     
     Parameter hash : forall `{H : State.Trait},
-        ref (Slice u8) ->
+        ref Slice ->
         mut_ref ink_env.hash.HashOutput.Type ->
         M (H := H) unit.
     
@@ -14557,7 +14551,7 @@ Module impls.
     Definition Self := ink_env.hash.Keccak256.
     
     Parameter hash : forall `{H : State.Trait},
-        ref (Slice u8) ->
+        ref Slice ->
         mut_ref ink_env.hash.HashOutput.Type ->
         M (H := H) unit.
     
@@ -14678,7 +14672,7 @@ Module impls.
     
     Parameter get_property : forall `{H : State.Trait},
         mut_ref Self ->
-        (ref ink_engine.ext.Engine) -> (mut_ref (mut_ref (Slice u8))) -> unit ->
+        (ref ink_engine.ext.Engine) -> (mut_ref (mut_ref Slice)) -> unit ->
         M (H := H) (ink_env.error.Result T).
     
     Global Instance Method_get_property `{H : State.Trait} :
@@ -14774,7 +14768,7 @@ Module impls.
     
     Parameter hash_bytes : forall `{H : State.Trait},
         mut_ref Self ->
-        ref (Slice u8) ->
+        ref Slice ->
         mut_ref ink_env.hash.HashOutput.Type ->
         M (H := H) unit.
     
@@ -14832,7 +14826,7 @@ Module impls.
     
     Parameter set_code_hash : forall `{H : State.Trait},
         mut_ref Self ->
-        ref (Slice u8) ->
+        ref Slice ->
         M (H := H) (ink_env.error.Result unit).
     
     Global Instance Method_set_code_hash `{H : State.Trait} :
@@ -15188,7 +15182,7 @@ Module Impl_ink_env_hash_CryptoHash_for_ink_env_hash_Blake2x128.
   Definition Self := ink_env.hash.Blake2x128.
   
   Parameter hash : forall `{H : State.Trait},
-      ref (Slice u8) ->
+      ref Slice ->
       mut_ref ink_env.hash.HashOutput.Type ->
       M (H := H) unit.
   
@@ -15251,14 +15245,14 @@ Parameter assert_type_eq_all : forall `{H : State.Trait},
 Parameter as_array : forall `{H : State.Trait},
     forall
     {T : Set},
-    mut_ref (Slice T) ->
+    mut_ref Slice ->
     M (H := H) (mut_ref list T).
 
 Module Impl_ink_env_hash_CryptoHash_for_ink_env_hash_Blake2x256.
   Definition Self := ink_env.hash.Blake2x256.
   
   Parameter hash : forall `{H : State.Trait},
-      ref (Slice u8) ->
+      ref Slice ->
       mut_ref ink_env.hash.HashOutput.Type ->
       M (H := H) unit.
   
@@ -15321,14 +15315,14 @@ Parameter assert_type_eq_all : forall `{H : State.Trait},
 Parameter as_array : forall `{H : State.Trait},
     forall
     {T : Set},
-    mut_ref (Slice T) ->
+    mut_ref Slice ->
     M (H := H) (mut_ref list T).
 
 Module Impl_ink_env_hash_CryptoHash_for_ink_env_hash_Sha2x256.
   Definition Self := ink_env.hash.Sha2x256.
   
   Parameter hash : forall `{H : State.Trait},
-      ref (Slice u8) ->
+      ref Slice ->
       mut_ref ink_env.hash.HashOutput.Type ->
       M (H := H) unit.
   
@@ -15391,14 +15385,14 @@ Parameter assert_type_eq_all : forall `{H : State.Trait},
 Parameter as_array : forall `{H : State.Trait},
     forall
     {T : Set},
-    mut_ref (Slice T) ->
+    mut_ref Slice ->
     M (H := H) (mut_ref list T).
 
 Module Impl_ink_env_hash_CryptoHash_for_ink_env_hash_Keccak256.
   Definition Self := ink_env.hash.Keccak256.
   
   Parameter hash : forall `{H : State.Trait},
-      ref (Slice u8) ->
+      ref Slice ->
       mut_ref ink_env.hash.HashOutput.Type ->
       M (H := H) unit.
   
@@ -15461,7 +15455,7 @@ Parameter assert_type_eq_all : forall `{H : State.Trait},
 Parameter as_array : forall `{H : State.Trait},
     forall
     {T : Set},
-    mut_ref (Slice T) ->
+    mut_ref Slice ->
     M (H := H) (mut_ref list T).
 
 Module Impl_core_convert_From_for_ink_env_error_Error.
@@ -15568,7 +15562,7 @@ Module Impl_ink_env_engine_off_chain_EnvInstance_4.
   
   Parameter get_property : forall `{H : State.Trait},
       mut_ref Self ->
-      (ref ink_engine.ext.Engine) -> (mut_ref (mut_ref (Slice u8))) -> unit ->
+      (ref ink_engine.ext.Engine) -> (mut_ref (mut_ref Slice)) -> unit ->
       M (H := H) (ink_env.error.Result T).
   
   Global Instance Method_get_property `{H : State.Trait} :
@@ -15663,7 +15657,7 @@ Module Impl_ink_env_backend_EnvBackend_for_ink_env_engine_off_chain_EnvInstance.
   
   Parameter hash_bytes : forall `{H : State.Trait},
       mut_ref Self ->
-      ref (Slice u8) ->
+      ref Slice ->
       mut_ref ink_env.hash.HashOutput.Type ->
       M (H := H) unit.
   
@@ -15721,7 +15715,7 @@ Module Impl_ink_env_backend_EnvBackend_for_ink_env_engine_off_chain_EnvInstance.
   
   Parameter set_code_hash : forall `{H : State.Trait},
       mut_ref Self ->
-      ref (Slice u8) ->
+      ref Slice ->
       M (H := H) (ink_env.error.Result unit).
   
   Global Instance Method_set_code_hash `{H : State.Trait} :
@@ -17175,7 +17169,7 @@ Module hash.
       hash
         `{H : State.Trait}
         :
-        (ref (Slice u8)) ->
+        (ref Slice) ->
         (mut_ref ink_env.hash.HashOutput.Type) ->
         (M (H := H) unit);
     }.
@@ -17652,7 +17646,7 @@ Module CryptoHash.
     hash
       `{H : State.Trait}
       :
-      (ref (Slice u8)) ->
+      (ref Slice) ->
       (mut_ref ink_env.hash.HashOutput.Type) ->
       (M (H := H) unit);
   }.
@@ -19226,7 +19220,7 @@ Module topics.
   Module PrefixedValue.
     Unset Primitive Projections.
     Record t : Set := {
-      prefix : ref (Slice u8);
+      prefix : ref Slice;
       value : ref T;
     }.
     Global Set Primitive Projections.
@@ -20400,7 +20394,7 @@ End Topics.
 Module PrefixedValue.
   Unset Primitive Projections.
   Record t : Set := {
-    prefix : ref (Slice u8);
+    prefix : ref Slice;
     value : ref T;
   }.
   Global Set Primitive Projections.
